ok

SStructTT/Static/Progress.lean
@@ -4,129 +4,76 @@ open ARS
 namespace Static
 variable {Srt : Type} [inst : SStruct Srt]
 
-inductive Value : Tm Srt -> Prop where
-  | srt s i : Value (.srt s i)
-  | pi A B r s : Value (.pi A B r s)
-  | lam A m r s : Value (.lam A m r s)
-  | sig A B r s : Value (.sig A B r s)
-  | tup m n r s :
-    Value m ->
-    (r = .ex -> Value n) ->
-    Value (.tup m n r s)
-  | bool : Value .bool
-  | tt : Value .tt
-  | ff : Value .ff
-  | idn A m n : Value (.idn A m n)
-  | rfl m : Value (.rfl m)
-
 lemma Typed.pi_canonical {A B C m : Tm Srt} {r s} :
     [] ⊢ m : C -> C === .pi A B r s -> Value m ->
     ∃ A n, m = .lam A n r s := by
   generalize e: [] = Γ
-  intro ty; induction ty generalizing A B s
-  all_goals try (intro eq vl; false_conv)
-  case var hs _ => subst_vars; cases hs
+  intro ty eq vl; induction ty <;> try trivial
+  all_goals try false_conv
   case lam A0 B0 m _ _ _ _ _ _ _ _ =>
     have ⟨_, _, _, _⟩ := Conv.pi_inj eq
     subst_vars; exists A0, m
-  case app => cases vl
-  case proj => cases vl
-  case ite => cases vl
-  case rw => cases vl
   case conv ihm _ =>
-    apply ihm
-    . assumption
-    . apply Conv.trans <;> assumption
-    . assumption
-  all_goals trivial
+    apply ihm <;> try assumption
+    apply Conv.trans <;> assumption
 
 lemma Typed.sig_canonical {A B C m : Tm Srt} {r s} :
     [] ⊢ m : C -> C === .sig A B r s -> Value m ->
     ∃ m1 m2, m = .tup m1 m2 r s := by
   generalize e: [] = Γ
-  intro ty; induction ty generalizing A B s
-  all_goals try (intro eq vl; false_conv)
-  case var hs _ => subst_vars; cases hs
-  case app => cases vl
+  intro ty eq vl; induction ty <;> try trivial
+  all_goals try false_conv
   case tup A0 B0 m n _ _ _ _ _ _ _ _ _ =>
     have ⟨_, _, _, _⟩ := Conv.sig_inj eq
     subst_vars; exists m, n
-  case proj => cases vl
-  case ite => cases vl
-  case rw => cases vl
   case conv ihm _ =>
-    apply ihm
-    . assumption
-    . apply Conv.trans <;> assumption
-    . assumption
-  all_goals trivial
+    apply ihm <;> try assumption
+    apply Conv.trans <;> assumption
 
 lemma Typed.bool_canonical {C m : Tm Srt} :
     [] ⊢ m : C -> C === .bool -> Value m -> m = .tt ∨ m = .ff := by
   generalize e: [] = Γ
-  intro ty; induction ty
-  all_goals try (intro eq vl; false_conv)
-  case var hs _ => subst_vars; cases hs
-  case app => cases vl
-  case proj => cases vl
-  case tt => left; rfl
-  case ff => right; rfl
-  case ite => cases vl
-  case rw => cases vl
+  intro ty eq vl; induction ty <;> try trivial
+  all_goals try false_conv
+  case tt => simp
+  case ff => simp
   case conv ihm _ =>
-    apply ihm
-    . assumption
-    . apply Conv.trans <;> assumption
-    . assumption
-  all_goals trivial
+    apply ihm <;> try assumption
+    apply Conv.trans <;> assumption
 
 lemma Typed.idn_canonical {A C m a b : Tm Srt} :
     [] ⊢ m : C -> C === .idn A a b -> Value m -> ∃ n, m = .rfl n := by
   generalize e: [] = Γ
-  intro ty; induction ty
-  all_goals try (intro eq vl; false_conv)
-  case var hs _ => subst_vars; cases hs
-  case app => cases vl
-  case proj => cases vl
-  case ite => cases vl
+  intro ty eq vl; induction ty <;> try trivial
+  all_goals try false_conv
   case rfl m _ _ => exists m
-  case rw => cases vl
   case conv ihm _ =>
-    apply ihm
-    . assumption
-    . apply Conv.trans <;> assumption
-    . assumption
-  all_goals trivial
+    apply ihm <;> try assumption
+    apply Conv.trans <;> assumption
 
 theorem Typed.progress {m A : Tm Srt} :
     [] ⊢ m : A -> (∃ n, m ~> n) ∨ Value m := by
   generalize e: [] = Γ
-  intro ty; induction ty
-  all_goals try trivial
+  intro ty; induction ty <;> (subst_vars; simp_all; try trivial)
   case srt => right; constructor
-  case var hs _ => subst_vars; cases hs
   case pi => right; constructor
   case lam => right; constructor
-  case app _ n r _ tym tyn ihm ihn =>
-    subst_vars
-    match ihm (Eq.refl _) with
+  case app n r _ tym tyn ihm ihn =>
+    match ihm with
     | .inl ⟨m, _⟩ =>
       left; exists Tm.app m n r
       constructor; assumption
     | .inr vl =>
       have ⟨A, m, _⟩ := tym.pi_canonical Conv.R vl
-      subst_vars
-      left; exists m.[n/]
-      constructor
+      subst_vars; left; exists m.[n/]; constructor
   case sig => right; constructor
   case tup m n r s _ _ _ _ _ ihm ihn =>
-    subst_vars
-    match ihm (Eq.refl _) with
+    match ihm with
     | .inl ⟨m, _⟩ =>
       left; exists Tm.tup m n r s
       constructor; assumption
     | .inr vl =>
-      match ihn (Eq.refl _) with
+      match ihn with
       | .inl ⟨n, _⟩ =>
         left; exists Tm.tup m n r s
         constructor; assumption
@@ -134,23 +81,19 @@ theorem Typed.progress {m A : Tm Srt} :
         right; constructor
         . assumption
         . intro; assumption
-  case proj C m n r _ _ _ _ tym _ _ ihm _ =>
-    subst_vars
-    match ihm (Eq.refl _) with
+  case proj C m n r _ _ _ _ tym _ ihm =>
+    match ihm with
     | .inl ⟨m, _⟩ =>
       left; exists Tm.proj C m n r
       constructor; assumption
     | .inr vl =>
       have ⟨m1, m2, _⟩ := tym.sig_canonical Conv.R vl
-      subst_vars
-      left; exists n.[m2,m1/]
-      constructor
+      subst_vars; left; exists n.[m2,m1/]; constructor
   case bool => right; constructor
   case tt => right; constructor
   case ff => right; constructor
-  case ite A m n1 n2 _ _ _ tym _ _ _ ihm _ _ =>
-    subst_vars
-    match ihm (Eq.refl _) with
+  case ite A m n1 n2 _ _ _ tym _ _ ihm _ _ =>
+    match ihm with
     | .inl ⟨m, _⟩ =>
       left; exists Tm.ite A m n1 n2
       constructor; assumption
@@ -160,15 +103,11 @@ theorem Typed.progress {m A : Tm Srt} :
       | inr => subst_vars; left; exists n2; constructor
   case idn => right; constructor
   case rfl => right; constructor
-  case rw A _ m n _ _ _ _ _ _ tyn _ _ ihn =>
-    subst_vars
-    match ihn (Eq.refl _) with
+  case rw A B m n _ _ _ _ _ _ tyn _ ihn =>
+    match ihn with
     | .inl ⟨n, _⟩ =>
       left; exists Tm.rw A m n
       constructor; assumption
     | .inr vl =>
       have ⟨_, _⟩ := Typed.idn_canonical tyn Conv.R vl
-      subst_vars
-      left; exists m
-      constructor
-  case conv => subst_vars; aesop
+      subst_vars; left; exists m; constructor
