SStructTT/Dynamic/Progress.lean
@@ -1,0 +1,146 @@
+import SStructTT.Static.Progress
+import SStructTT.Dynamic.Step
+import SStructTT.Dynamic.Inversion
+open ARS Static
+
+namespace Dynamic
+variable {Srt : Type} [inst : SStruct Srt]
+
+lemma Typed.pi_canonical {A B C m : Tm Srt} {r s} :
+    [] ;; [] ⊢ m : C -> C === .pi A B r s -> Value m ->
+    ∃ A n, m = .lam A n r s := by
+  generalize e1: [] = Γ
+  generalize e2: [] = Δ
+  intro ty eq vl; induction ty <;> try trivial
+  all_goals try false_conv
+  case lam_im A B m _ _ _ _ _ _ _  =>
+    have ⟨_, _, eqA, eqB⟩ := Conv.pi_inj eq
+    subst_vars; exists A, m
+  case lam_ex A B m _ _ _ _ _ _ _ _ _ =>
+    have ⟨_, _, eqA, eqB⟩ := Conv.pi_inj eq
+    subst_vars; exists A, m
+  case conv ih =>
+    apply ih <;> try assumption
+    apply Conv.trans <;> assumption
+
+lemma Typed.sig_canonical {A B C m : Tm Srt} {r s} :
+    [] ;; [] ⊢ m : C -> C === .sig A B r s -> Value m ->
+    ∃ m1 m2, m = .tup m1 m2 r s := by
+  generalize e1: [] = Γ
+  generalize e2: [] = Δ
+  intro ty eq vl; induction ty <;> try trivial
+  all_goals try false_conv
+  case tup_im A0 B0 m n _ _ _ _ _ _ =>
+    have ⟨_, _, _, _⟩ := Conv.sig_inj eq
+    subst_vars; exists m, n
+  case tup_ex A0 B0 m n _ _ _ _ _ _ _ _ =>
+    have ⟨_, _, _, _⟩ := Conv.sig_inj eq
+    subst_vars; exists m, n
+  case conv ihm =>
+    apply ihm <;> try assumption
+    apply Conv.trans <;> assumption
+
+lemma Typed.bool_canonical {C m : Tm Srt} :
+    [] ;; [] ⊢ m : C -> C === .bool -> Value m -> m = .tt ∨ m = .ff := by
+  generalize e1: [] = Γ
+  generalize e2: [] = Γ
+  intro ty eq vl; induction ty <;> try trivial
+  all_goals try false_conv
+  case tt => simp
+  case ff => simp
+  case conv ihm =>
+    apply ihm <;> try assumption
+    apply Conv.trans <;> assumption
+
+lemma Typed.idn_canonical {A C m a b : Tm Srt} :
+    [] ;; [] ⊢ m : C -> C === .idn A a b -> Value m -> ∃ n, m = .rfl n := by
+  generalize e1: [] = Γ
+  generalize e2: [] = Δ
+  intro ty eq vl; induction ty <;> try trivial
+  all_goals try false_conv
+  case conv ihm =>
+    apply ihm <;> try assumption
+    apply Conv.trans <;> assumption
+
+theorem Typed.progress {m A : Tm Srt} :
+    [] ;; [] ⊢ m : A -> (∃ n, m ~>> n) ∨ Value m := by
+  generalize e1: [] = Γ
+  generalize e2: [] = Δ
+  intro ty; induction ty <;> (subst_vars; simp_all; try trivial)
+  case lam_im => right; constructor
+  case lam_ex => right; constructor
+  case app_im n _ _ tym ih =>
+    match ih with
+    | .inl ⟨m, _⟩ =>
+      left; exists Tm.app m n .im
+      constructor; assumption
+    | .inr vl =>
+      have ⟨_, m, _⟩ := tym.pi_canonical Conv.R vl
+      subst_vars; left; exists m.[n/]; constructor
+  case app_ex m n _ tym tyn ihm ihn mrg =>
+    cases mrg; simp_all
+    match ihm with
+    | .inl ⟨m, _⟩ =>
+      left; exists Tm.app m n .ex
+      constructor; assumption
+    | .inr vl =>
+      match ihn with
+      | .inl ⟨n, _⟩ =>
+        left; exists Tm.app m n .ex
+        constructor; assumption
+      | .inr _ =>
+        have ⟨_, m, _⟩ := tym.pi_canonical Conv.R vl
+        subst_vars; left; exists m.[n/]
+        constructor; assumption
+  case tup_im m n s _ _ _ _ ih =>
+    match ih with
+    | .inl ⟨m, _⟩ =>
+      left; exists Tm.tup m n .im s
+      constructor; assumption
+    | .inr _ => right; constructor; assumption
+  case tup_ex m n s _ _ _ _ ihm ihn mrg =>
+    cases mrg; simp_all
+    match ihm with
+    | .inl ⟨m, _⟩ =>
+      left; exists Tm.tup m n .ex s
+      constructor; assumption
+    | .inr _ =>
+      match ihn with
+      | .inl ⟨n, _⟩ =>
+        left; exists Tm.tup m n .ex s
+        constructor; assumption
+      | .inr _ => right; constructor <;> assumption
+  case proj_im C _ n _ _ _ _ _ _ _ _ tym _ ihm mrg =>
+    cases mrg; simp_all
+    match ihm with
+    | .inl ⟨m, _⟩ =>
+      left; exists Tm.proj C m n .im
+      constructor; assumption
+    | .inr vl =>
+      have ⟨m1, m2, _⟩ := tym.sig_canonical Conv.R vl
+      subst_vars; left; exists n.[m2,m1/]
+      constructor; assumption
+  case proj_ex C _ n _ _ _ _ _ _ _ _ _ _ tym _ ihm mrg =>
+    cases mrg; simp_all
+    match ihm with
+    | .inl ⟨m, _⟩ =>
+      left; exists Tm.proj C m n .ex
+      constructor; assumption
+    | .inr vl =>
+      have ⟨m1, m2, _⟩ := tym.sig_canonical Conv.R vl
+      subst_vars; left; exists n.[m2,m1/]
+      constructor; assumption
+  case tt => right; constructor
+  case ff => right; constructor
+  case ite A _ n1 n2 _ _ _ tym _ _ ihm _ _ mrg =>
+    cases mrg; simp_all
+    match ihm with
+    | .inl ⟨m, _⟩ =>
+      left; exists Tm.ite A m n1 n2
+      constructor; assumption
+    | .inr vl =>
+      cases tym.bool_canonical Conv.R vl with
+      | inl => subst_vars; left; exists n1; constructor
+      | inr => subst_vars; left; exists n2; constructor
+  case rw m n _ _ _ _ _ _ _ _ =>
+    left; exists m; constructor
